src/SDK/CMM/Defs.dfy
@@ -2,6 +2,7 @@ include "../Materials.dfy"
 include "../../StandardLibrary/StandardLibrary.dfy"
 include "../../StandardLibrary/UInt.dfy"
 include "../../Crypto/Signature.dfy"
+include "../MessageHeader.dfy"
 
 module CMMDefs {
   import opened StandardLibrary
@@ -9,6 +10,7 @@ module CMMDefs {
   import Materials
   import AlgorithmSuite
   import Signature
+  import MessageHeader
 
   trait {:termination false} CMM {
     ghost var Repr : set<object>
@@ -24,12 +26,19 @@ module CMMDefs {
                                res.value.plaintextDataKey.Some? && 
                                |res.value.plaintextDataKey.get| == res.value.algorithmSuiteID.KDFInputKeyLength() &&
                                |res.value.encryptedDataKeys| > 0
+      ensures res.Success? ==> ValidAAD(res.value.encryptionContext)
       ensures res.Success? ==>
         match res.value.algorithmSuiteID.SignatureType()
           case None => true
           case Some(sigType) =>
             res.value.signingKey.Some? &&
             Signature.ECDSA.WfSK(sigType, res.value.signingKey.get)
+
+    // The following predicate is a synonym for MessageHeader.ValidAAD and provides a workaround for a translation bug
+    // of "fuel" in trait-override checks in Dafny.
+    predicate ValidAAD(encryptionContext: Materials.EncryptionContext) {
+      MessageHeader.ValidAAD(encryptionContext)
+    }
 
     method DecryptMaterials(algSuiteID: AlgorithmSuite.ID,
                             edks: seq<Materials.EncryptedDataKey>,
