src/Main.dfy
@@ -29,9 +29,18 @@ module Main {
     var msg := UTF8.Encode("hello").value;
     print "Original plaintext: ", msg, "\n";
 
-    var encryptionContext := [];
+    var keyA, valA := UTF8.Encode("keyA").value, UTF8.Encode("valA").value;
+    var encryptionContext := [(keyA, valA)];
     assert Msg.ValidAAD(encryptionContext) by {
+      // To proving ValidAAD, we need to reveal the definition of ValidAAD:
       reveal Msg.ValidAAD();
+      // We also need to help the verifier with proving the AADLength is small:
+      calc {
+        Msg.AADLength(encryptionContext);
+        2 + Msg.KVPairsLength(encryptionContext, 0, 1);
+        2 + 2 + |keyA| + 2 + |valA|;
+      }
+      assert Msg.AADLength(encryptionContext) < UINT16_LIMIT;
     }
     var e := Client.Encrypt(msg, cmm, encryptionContext);
     if e.Failure? {
